Base Case ($n=0$): 
$\sum_{j=0}^{0} j \cdot 3^{j} = 0 \cdot 3^0 = 0$

Now, let's check the right side of the equation for n=0: 
$\frac{3}{4}[ 0\cdot3^{0+1} - (0+1)3^0 + 1] = \frac{3}{4}[0 - 3^0 + 1] = \frac{3}{4}[-1 + 1] = 0$

Since both sides of the equation are equal, the base case holds.

Inductive Step: Assume the statement is true for $n=k$:
$\sum_{j=0}^{k} j \cdot 3^{j} = \frac{3}{4}[ k\cdot3^{k+1} - (k+1)3^k + 1]$

Now, we must prove that the statement is true for $n=k+1$: 
$\sum_{j=0}^{k+1} j \cdot 3^{j} = \sum_{j=0}^{k} j \cdot 3^{j} + (k+1) \cdot 3^{k+1}$

By using the inductive hypothesis, we can substitute the sum for n=k: 
$\sum_{j=0}^{k+1} j \cdot 3^{j} = \frac{3}{4}[ k\cdot3^{k+1} - (k+1)3^k + 1] + (k+1) \cdot 3^{k+1}$

Now, let's simplify and rearrange the terms: 
$= \frac{3}{4}[k\cdot3^{k+1}] - \frac{3}{4}[(k+1)3^k] + \frac{3}{4}[1] + (k+1) \cdot 3^{k+1}$

Combine the terms with a common factor of $(k+1)3^{k+1}$: 
$= \frac{3}{4}[k\cdot3^{k+1}] + (k+1) \cdot 3^{k+1}(1 - \frac{3}{4}) + \frac{3}{4}[1]$

$= \frac{3}{4}[k\cdot3^{k+1}] + (k+1) \cdot 3^{k+1}(\frac{1}{4}) + \frac{3}{4}[1]$

Factor out $3^{k+1}$: 
$= \frac{3}{4}[(k+1)3^{k+1} - k\cdot3^{k+1}] + \frac{3}{4}[1]$

$= \frac{3}{4}[(k+1)3^{k+1} - k\cdot3^{k+1} + 3^0]$

Now, let's check if it matches the right side of the equation for n=k+1: 
$\frac{3}{4}[ (k+1)\cdot3^{(k+1)+1} - ((k+1)+1)3^{k+1} + 1]$

$= \frac{3}{4}[ (k+1)\cdot3^{k+2} - (k+2)3^{k+1}$




$= \frac{3}{4}[k\cdot3^{k+1}] - \frac{3}{4}[(k+1)3^k] + \frac{3}{4}[1] + (k+1) \cdot 3^{k+1}$

$= 3^{k+1}(k+1)(\frac{7}{4}) - (k+1)3^k(\frac{3}{4}) + \frac{3}{4}$
