
Proof of Onto and One-to-One

$$
	\displaylines{
		∀x_1∀x_2[f(x_1) = f(x_2) → x_1 = x_2] \\ \\
		y = f(x) = e^x \\ \\
		ln(y) = ln(e^x) = x \\ \\
		e^{x_1} = e^{x_2} => ln(e^{x_1}) = ln(e^{x_2}) = x_1 = x_2
	}
$$


$$
\displaylines{
	n = p \cdot b^t \Leftrightarrow \frac n p = b^t \\
	∴ ~~~ \log_b (\frac n p) = t
	
}
$$

## after class notes
1. Theorem: if a, b, and c are integers such that a^3|b and b^2|c then a^6|c

(p ∧ q ) → r

a^3|b => b = ka^3   k∈z
b^2|c => c = jb^2    j :∈z

= j(ka^3)^2 = (jk^2)a^6 = la^6 => means c is divisible by a^6.

2. Theorem: xy|z → (x|z ∧ y|z)

x ∈ Z
y ∈ Z
z ∈ Z

z = k(xy)    k ∈ Z

(ky)x = (l)x  => z is divisible by x => x|z
(kx)y = (m)y => z is divisible by y => y|z

3. Theorem (5n+3 = 2k) → (n=2l+1) ≡ ¬q → ¬p

5n+3 is even, because of 2k.
n is odd, because of 2l + 1.

(¬q→¬p) ≡ ((n = 2l) → (5n + 3 = 2k + 1))

5n+3 = 5(2l) + 3 = 10l + 3 = 10l + 2 + 1 = 2(5l+1) + 1 

= 2m + 1  where m ∈ Z

4.  3∤xy → 3∤x

By contrapositive:
¬q → ¬p

(3|n) → (3|xy)

x = 3k → xy=3m
k ∈ Z   and m ∈ Z

xy = (3k)y = 3(ky) = 3m